refactor: use the Equality typeclass for addresses
With the Equality typeclass, the main idea is to rely as much
as possible on a unified interface for equalities. The addresses
are the first SpecCert component to use them as much as possible.

src/Address/PhysicalAddress.v
@@ -6,6 +6,7 @@ Require Import SpecCert.Address.AddressSpace.
 Require Import SpecCert.Address.Address.
 Require Import SpecCert.Interval.
 Require Import SpecCert.Utils.
+Require Import SpecCert.Equality.
 
 (**
    Definition
@@ -14,37 +15,70 @@ Require Import SpecCert.Utils.
 Inductive MemoryMap :=
 | mm: MemoryMap.
 
-Lemma memory_map_singleton: forall m m': MemoryMap, m = m'.
+Lemma mm_singleton: forall m m': MemoryMap, m = m'.
 Proof.
   induction m; induction m'; reflexivity.
 Qed.
 
-Definition mm_eq: relation MemoryMap :=
-  fun (m m': MemoryMap) => True.
+Definition mm_eq
+           (m m': MemoryMap)
+  : Prop :=
+  m = m'.
 
-Definition mm_eq_dec: forall (m m': MemoryMap), {m = m'}+{m <> m'}.
-  decide equality.
+Definition mm_eq_dec
+           (m m': MemoryMap)
+  : {mm_eq m m'}+{~ mm_eq m m'}.
+  left.
+  apply mm_singleton.
 Defined.
 
-Lemma mm_eq_refl: forall m: MemoryMap, mm_eq m m.
+Lemma mm_eq_refl
+      (m: MemoryMap)
+  : mm_eq m m.
 Proof.
   unfold mm_eq; auto.
 Qed.
 
-Lemma mm_eq_sym: forall m m': MemoryMap, mm_eq m m' -> mm_eq m' m.
+Lemma mm_eq_sym
+      (m m': MemoryMap)
+  : mm_eq m m' -> mm_eq m' m.
 Proof.
   unfold mm_eq; auto.
 Qed.
 
-Lemma mm_eq_trans:
-  forall (m m' m'': MemoryMap),
-    mm_eq m m'
+Lemma mm_eq_trans
+      (m m' m'': MemoryMap)
+  : mm_eq m m'
     -> mm_eq m' m''
     -> mm_eq m m''.
 Proof.
-  intros m m' m''; rewrite (memory_map_singleton m' m); rewrite (memory_map_singleton m'' m).
+  rewrite (mm_singleton m' m); rewrite (mm_singleton m'' m).
   trivial.
 Qed.
+
+Lemma mm_eq_eq
+      (m m': MemoryMap)
+  : mm_eq m m' -> m = m'.
+unfold mm_eq; auto.
+Qed.
+
+Lemma eq_mm_eq
+      (m m': MemoryMap)
+  : m = m' -> mm_eq m m'.
+Proof.
+  intro Heq.
+  apply mm_singleton.
+Qed.
+
+Instance memoryMapEq : Eq MemoryMap :=
+  { eq       := mm_eq
+  ; eq_refl  := mm_eq_refl
+  ; eq_sym   := mm_eq_sym
+  ; eq_trans := mm_eq_trans
+  ; eq_dec   := mm_eq_dec
+  ; eq_equal := mm_eq_eq
+  ; equal_eq := eq_mm_eq
+  }.
 
 Definition PhysicalAddress := Address MemoryMap.
 
@@ -69,5 +103,5 @@ Defined.
 Definition phys_addr_eq_dec
            (pa pa': PhysicalAddress)
   : {addr_eq pa pa'}+{~ addr_eq pa pa'}.
-refine (decide_dec (addr_eq_dec mm_eq_dec pa pa')); trivial.
+refine (decide_dec (addr_eq_dec pa pa')); trivial.
 Defined.
