src/Memory/Memory_func.v
@@ -1,12 +1,13 @@
 Require Import SpecCert.Address.
 Require Import SpecCert.Memory.Memory_def.
+Require Import SpecCert.Map.
 
 Definition find_in_memory
            {S   :Set}
            (mem :Memory S)
            (ha  :HardwareAddress)
            :S :=
-  _HardAddrMap.find_in_map mem ha.
+  find_in_map mem ha.
 
 Definition update_in_memory
            {S      :Set}
@@ -14,4 +15,4 @@ Definition update_in_memory
            (ha     :HardwareAddress)
            (owner :S)
            :Memory S :=
-  _HardAddrMap.add_in_map mem ha owner.
+  add_in_map mem ha owner.
